Add decl hashcons, decl equality, implement [create_data_decl]

extract/DeclExn.ml
@@ -1,3 +1,16 @@
 exception UnboundVar of vsymbol
 exception UnexpectedProjOrConstr of lsymbol
 exception NoTerminationProof of lsymbol
+
+exception IllegalTypeAlias of tysymbol
+exception ClashIdent of ident
+exception BadConstructor of lsymbol
+
+exception BadRecordField of lsymbol
+exception RecordFieldMissing of lsymbol
+exception DuplicateRecordField of lsymbol
+
+exception EmptyDecl
+exception EmptyAlgDecl of tysymbol
+
+exception NonPositiveTypeDecl of tysymbol * lsymbol * ty
