src/core/DeclDefs.v
@@ -1,4 +1,6 @@
-Require Import CoqInt TyDefs TermDefs IdentDefs.
+Require Import CoqInt TyDefs TermDefs TermFuncs IdentDefs CoqWstdlib.
+Import MonadNotations.
+Set Bullet Behavior "Strict Subproofs".
 
 (*JOSH TODO: HORRIBLE HACK*)
 (*Coq's extraction does not know that tysymbol_c -> tysymbol_o
@@ -28,10 +30,32 @@ Definition logic_decl : Type := lsymbol * ls_defn.
 (* Inductive Predicate declaration *)
 Record prsymbol := { pr_name : ident }.
 
-(*TODO: Spr, Mpr, etc*)
-(*TODO: pr_equal, pr_hash, create_prsymbol*)
+Definition prsymbol_eqb (p1 p2: prsymbol) : bool :=
+  id_equal p1.(pr_name) p2.(pr_name).
 
-Definition ind_decl : Type := lsymbol * list (prsymbol * term).
+Lemma prsymbol_eqb_eq p1 p2: p1 = p2 <-> prsymbol_eqb p1 p2.
+Proof.
+  destruct p1 as [i1]; destruct p2 as [i2]; unfold prsymbol_eqb; simpl.
+  rewrite <- ident_eqb_eq. solve_eqb_eq.
+Qed.
+
+Module PropTag <: TaggedType.
+Definition t := prsymbol.
+Definition tag pr := pr.(pr_name).(id_tag).
+Definition equal := prsymbol_eqb.
+End PropTag.
+
+Module Prop1 := MakeMSWeak PropTag.
+Module Spr := Prop1.S.
+Module Mpr := Prop1.M.
+
+Definition pr_equal := prsymbol_eqb.
+Definition pr_hash pr := id_hash pr.(pr_name).
+Definition create_prsymbol n : ctr prsymbol := 
+  (i <- id_register n ;;
+  st_ret {| pr_name := i |})%state.
+
+Definition ind_decl : Type := lsymbol * list (prsymbol * term_c).
 
 (*TODO: we do not support Coind*)
 Variant ind_sign := Ind | Coind.
@@ -45,9 +69,7 @@ Variant prop_kind :=
   | Pgoal (*prove, do not use as premise*)
   .
 
-(*TODO: MOVE*)
-
-Definition prop_decl : Type := ocaml_tup3 prop_kind prsymbol term.
+Definition prop_decl : Type := ocaml_tup3 prop_kind prsymbol term_c.
 
 (* Declaration Type *)
 
@@ -60,18 +82,59 @@ Variant decl_node :=
   | Dprop : prop_decl -> decl_node (*axiom/lemma/goal*)
   .
 
-Record decl := mk_decl { 
+Record decl := build_decl { 
   d_node : decl_node;
   d_news : Sid.t;
   d_tag : CoqWeakhtbl.tag}.
 
 (*Decidable Equality*)
+Section Equality. 
+
 Definition constructor_eqb : constructor -> constructor -> bool :=
   tuple_eqb ls_equal (list_eqb (option_eqb ls_equal)).
 
 Definition data_decl_eqb : data_decl -> data_decl -> bool :=
   tuple_eqb ts_equal (list_eqb constructor_eqb).
 
+Scheme Equality for ind_sign.
+Scheme Equality for prop_kind.
+
+Definition ind_sign_eqb := ind_sign_beq.
+Definition prop_kind_eqb := prop_kind_beq.
+
+Definition ls_defn_eqb : ls_defn -> ls_defn -> bool :=
+  tuple_eqb (tuple_eqb ls_equal term_eqb) (list_eqb CoqBigInt.eqb).
+
+Definition logic_decl_eqb : logic_decl -> logic_decl -> bool :=
+  tuple_eqb ls_equal ls_defn_eqb.
+
+Definition ind_decl_eqb : ind_decl -> ind_decl -> bool :=
+  tuple_eqb ls_equal (list_eqb (tuple_eqb prsymbol_eqb term_eqb)).
+
+(*Almost the same as hashcons equivalent but not quite.
+  Hashcons does not care about all components of [logic_decl].
+  Also, we need strict equality and not equality modulo alpha equiv *)
+Definition decl_node_eqb (d1 d2: decl_node) : bool :=
+  match d1, d2 with
+  | Dtype s1, Dtype s2 => ts_equal s1 s2
+  | Ddata l1, Ddata l2 => list_eqb data_decl_eqb l1 l2
+  | Dparam s1, Dparam s2 => ls_equal s1 s2
+  | Dlogic l1, Dlogic l2 => list_eqb logic_decl_eqb l1 l2
+  | Dind (s1, l1), Dind (s2, l2) => ind_sign_eqb s1 s2 &&
+    list_eqb ind_decl_eqb l1 l2
+  | Dprop p1, Dprop p2 =>
+    let '(k1, pr1, f1) := of_tup3 p1 in
+    let '(k2, pr2, f2) := of_tup3 p2 in
+    prop_kind_eqb k1 k2 && pr_equal pr1 pr2 && term_eqb f1 f2
+  | _, _ => false
+  end.
+
+Definition decl_eqb (d1 d2: decl) : bool :=
+  decl_node_eqb d1.(d_node) d2.(d_node) &&
+  Sid.equal d1.(d_news) d2.(d_news) &&
+  CoqWeakhtbl.tag_equal d1.(d_tag) d2.(d_tag).
+
+(*And the proofs*) 
 Lemma constructor_eqb_eq c1 c2:
   c1 = c2 <-> constructor_eqb c1 c2.
 Proof.
@@ -87,3 +150,195 @@ Proof.
   - apply tysymbol_eqb_eq.
   - apply list_eqb_eq, constructor_eqb_eq.
 Qed.
+
+Lemma ind_sign_eqb_eq i1 i2:
+  i1 = i2 <-> ind_sign_eqb i1 i2.
+Proof.
+  split; intros.
+  - apply internal_ind_sign_dec_lb; auto.
+  - apply internal_ind_sign_dec_bl; auto.
+Qed.
+
+Lemma prop_kind_eqb_eq p1 p2:
+  p1 = p2 <-> prop_kind_eqb p1 p2.
+Proof.
+  split; intros.
+  - apply internal_prop_kind_dec_lb; auto.
+  - apply internal_prop_kind_dec_bl; auto.
+Qed.
+
+Lemma ls_defn_eqb_eq l1 l2:
+  l1 = l2 <-> ls_defn_eqb l1 l2.
+Proof.
+  apply tuple_eqb_spec.
+  - intros. apply tuple_eqb_spec.
+    + apply lsymbol_eqb_eq.
+    + apply term_eqb_eq.
+  - apply list_eqb_eq, CoqBigInt.eqb_eq.
+Qed. 
+
+Lemma logic_decl_eqb_eq l1 l2:
+  l1 = l2 <-> logic_decl_eqb l1 l2.
+Proof.
+  apply tuple_eqb_spec.
+  - apply lsymbol_eqb_eq.
+  - apply ls_defn_eqb_eq.
+Qed.
+
+Lemma ind_decl_eqb_eq i1 i2:
+  i1 = i2 <-> ind_decl_eqb i1 i2.
+Proof.
+  apply tuple_eqb_spec.
+  - apply lsymbol_eqb_eq.
+  - apply list_eqb_eq, tuple_eqb_spec.
+    + apply prsymbol_eqb_eq.
+    + apply term_eqb_eq.
+Qed.
+
+Lemma decl_node_eqb_eq d1 d2:
+  d1 = d2 <-> decl_node_eqb d1 d2.
+Proof.
+  destruct d1 as [| | | | i1 |p1]; destruct d2 as [| | | | i2 |p2]; unfold decl_node_eqb; simpl; 
+  try solve[solve_eqb_eq]; try solve[destruct i1; solve_eqb_eq];
+  [rewrite <- tysymbol_eqb_eq | 
+   rewrite <- (list_eqb_eq data_decl_eqb_eq) |
+   rewrite <- lsymbol_eqb_eq |
+   rewrite <- (list_eqb_eq logic_decl_eqb_eq) |
+   | ]; try solve[solve_eqb_eq].
+  - destruct i1; destruct i2.
+    rewrite andb_true, <- ind_sign_eqb_eq, <- (list_eqb_eq ind_decl_eqb_eq).
+    solve_eqb_eq.
+  - destruct (of_tup3 p1) as [[k1 pr1] f1] eqn : Htup1.
+    destruct (of_tup3 p2) as [[k2 pr2] f2] eqn : Htup2.
+    (*A bit trickier because we cannot break OCaml abstraction*)
+    rewrite !andb_true. rewrite <- prop_kind_eqb_eq, <- prsymbol_eqb_eq, <- term_eqb_eq.
+    (*Need to solve manually*)
+    split; intros Heq.
+    + inversion Heq; subst. rewrite Htup1 in Htup2. inversion Htup2; auto.
+    + destruct_all; subst.
+      f_equal. apply of_tup3_inj. rewrite Htup1, Htup2. reflexivity.
+Qed.
+
+Lemma decl_eqb_eq d1 d2:
+  d1 = d2 <-> decl_eqb d1 d2.
+Proof.
+  destruct d1 as [d1 s1 t1]. destruct d2 as [d2 s2 t2].
+  unfold decl_eqb; simpl.
+  rewrite !andb_true, <- decl_node_eqb_eq, <- Sid.equal_eq, 
+  (*TODO: breaks abstraction, add to CoqWeakhtbl*)
+  <- CoqBigInt.eqb_eq; [solve_eqb_eq |].
+  apply ident_eqb_eq.
+Qed.
+
+End Equality.
+
+(*Hash-consing*)
+Module DeclHash <: hashcons.HashedType.
+
+Definition t := decl.
+(*Weaker than structural equality; ignore tags and metadata*)
+
+Definition eq_ld (x1 x2: logic_decl) : bool :=
+  ls_equal (fst x1) (fst x2) &&
+  t_equal_strict (snd (fst (snd x1))) (snd (fst (snd x2))).
+
+Definition eq_iax :=
+  tuple_eqb pr_equal t_equal_strict.
+
+Definition eq_ind1 : ind_decl-> ind_decl -> bool :=
+  tuple_eqb ls_equal (list_eqb eq_iax).
+
+
+Definition equal (d1 d2: decl) : bool :=
+  match d1.(d_node), d2.(d_node) with
+  | Dtype s1, Dtype s2 => ts_equal s1 s2
+  | Ddata l1, Ddata l2 => list_eqb data_decl_eqb l1 l2
+  | Dparam s1, Dparam s2 => ls_equal s1 s2
+  | Dlogic l1, Dlogic l2 => list_eqb eq_ld l1 l2
+  | Dind (s1, l1), Dind (s2, l2) => ind_sign_eqb s1 s2 &&
+    list_eqb eq_ind1 l1 l2
+  | Dprop p1, Dprop p2 =>
+    let '(k1, pr1, f1) := of_tup3 p1 in
+    let '(k2, pr2, f2) := of_tup3 p2 in
+    prop_kind_eqb k1 k2 && pr_equal pr1 pr2 && t_equal_strict f1 f2
+  | _, _ => false
+  end.
+
+(*Hashing - similar*)
+Definition cs_hash (x: constructor) : CoqBigInt.t :=
+  hashcons.combine_big_list (hashcons.combine_big_option ls_hash) 
+    (ls_hash (fst x)) (snd x).
+
+Definition hs_td (x: data_decl) : CoqBigInt.t :=
+  hashcons.combine_big_list cs_hash (ts_hash (fst x)) (snd x).
+
+Definition hs_ld (x: logic_decl) : CoqBigInt.t :=
+  hashcons.combine_big (ls_hash (fst x)) (t_hash_strict (snd (fst (snd x)))).
+
+Definition hs_prop (x: prsymbol * term_c) : CoqBigInt.t :=
+  hashcons.combine_big (pr_hash (fst x)) (t_hash_strict (snd x)).
+
+Definition hs_ind (x: ind_decl) : CoqBigInt.t :=
+  hashcons.combine_big_list hs_prop (ls_hash (fst x)) (snd x).
+
+Definition hs_kind (p: prop_kind) : CoqBigInt.t :=
+  match p with
+  | Plemma => CoqBigInt.eleven
+  | Paxiom => CoqBigInt.thirteen
+  | Pgoal => CoqBigInt.seventeen
+  end.
+
+Definition hash (d: decl) : CoqBigInt.t :=
+  match d.(d_node) with
+  | Dtype s => ts_hash s
+  | Ddata l => hashcons.combine_big_list hs_td (CoqBigInt.three) l
+  | Dparam s => ls_hash s
+  | Dlogic l => hashcons.combine_big_list hs_ld CoqBigInt.five l
+  | Dind (_, l) => hashcons.combine_big_list hs_ind CoqBigInt.seven l
+  | Dprop y => let '(k, pr, f) := of_tup3 y in
+    hashcons.combine_big (hs_kind k) (hs_prop (pr, f))
+  end.
+
+Definition tag (n: CoqWeakhtbl.tag) (d: decl) : decl :=
+  {| d_node := d.(d_node); d_news := d.(d_news);
+    d_tag := (CoqWeakhtbl.create_tag n)|}.
+
+End DeclHash.
+
+Module Hsdecl := hashcons.Make DeclHash.
+
+Module DeclTag <: TaggedType.
+Definition t := decl.
+Definition tag d := d.(d_tag).
+(*TODO: We cannot use reference equality, but can we just
+  compare tags? TODO TRY THIS!
+  For now, use decidable equality, which is much slower*)
+Definition equal := decl_eqb.
+End DeclTag.
+
+Module Decl1 := MakeMSWeak DeclTag.
+Module Sdecl := Decl1.S.
+Module Mdecl := Decl1.M.
+
+(*TODO: see note above (note: it will make proofs harder,
+  we will have to expose both but we need to do anyway
+  e.g. for term)*)
+Definition d_equal := decl_eqb.
+Definition d_hash d := CoqWeakhtbl.tag_hash d.(d_tag).
+
+(*Declaration Constructors*)
+
+Definition mk_decl (node: decl_node) (news: Sid.t) : 
+  st (hashcons_ty decl) decl :=
+  let d := {| d_node := node; 
+    d_news := news; 
+    d_tag := CoqWeakhtbl.dummy_tag |} in
+  match node with
+  | Dprop p =>
+    let '(x, _, _) := of_tup3 p in
+    match x with
+    | Pgoal => Hsdecl.unique d
+    | _ => Hsdecl.hashcons d
+    end
+  | _ => Hsdecl.hashcons d
+  end.
